Extended the definition of a correct relation and filled 1/3 remaining holes

src/DenotationalSem.v
@@ -73,7 +73,7 @@ Inductive in_denotational_sem_goal : goal -> gt_fun -> Prop :=
                              in_denotational_sem_goal (Conj g1 g2) f
 | dsgFresh  : forall f fn a fg (fvH : ~ is_fv_of_goal a (Fresh fg))
                                (Hg : in_denotational_sem_goal (fg a) fn)
-                               (Hease : forall (x : name) (neq : x <> a), fn x = f x),
+                               (Hease : forall (x : name) (neq : x <> a), gt_eq (fn x) (f x)),
                                in_denotational_sem_goal (Fresh fg) f
 | dsgInvoke : forall r t f (Hbody : in_denotational_sem_goal (proj1_sig (MiniKanrenSyntax.P r) t) f),
                            in_denotational_sem_goal (Invoke r t) f.
@@ -82,20 +82,20 @@ Hint Constructors in_denotational_sem_goal.
 
 Inductive in_denotational_sem_lev_goal : nat -> goal -> gt_fun -> Prop :=
 | dslgUnify  : forall l f t1 t2 (UnH : gt_eq (apply_gt_fun f t1) (apply_gt_fun f t2)),
-                              in_denotational_sem_lev_goal (S l) (Unify t1 t2) f
+                                in_denotational_sem_lev_goal (S l) (Unify t1 t2) f
 | dslgDisjL  : forall l f g1 g2 (Hg :in_denotational_sem_lev_goal l g1 f),
-                               in_denotational_sem_lev_goal l (Disj g1 g2) f
+                                in_denotational_sem_lev_goal l (Disj g1 g2) f
 | dslgDisjR  : forall l f g1 g2 (Hg :in_denotational_sem_lev_goal l g2 f),
-                               in_denotational_sem_lev_goal l (Disj g1 g2) f
+                                in_denotational_sem_lev_goal l (Disj g1 g2) f
 | dslgConj   : forall l f g1 g2 (Hg1 :in_denotational_sem_lev_goal l g1 f)
                                 (Hg2 :in_denotational_sem_lev_goal l g2 f),
-                               in_denotational_sem_lev_goal l (Conj g1 g2) f
+                                in_denotational_sem_lev_goal l (Conj g1 g2) f
 | dslgFresh  : forall l f fn a fg (fvH : ~ is_fv_of_goal a (Fresh fg))
                                   (Hg :in_denotational_sem_lev_goal l (fg a) fn)
-                                  (Hease : forall (x : name) (neq : x <> a), fn x = f x),
-                                 in_denotational_sem_lev_goal l (Fresh fg) f
+                                  (Hease : forall (x : name) (neq : x <> a), gt_eq (fn x) (f x)),
+                                  in_denotational_sem_lev_goal l (Fresh fg) f
 | dslgInvoke : forall l r t f (Hbody :in_denotational_sem_lev_goal l (proj1_sig (MiniKanrenSyntax.P r) t) f),
-                             in_denotational_sem_lev_goal (S l) (Invoke r t) f.
+                              in_denotational_sem_lev_goal (S l) (Invoke r t) f.
 
 Hint Constructors in_denotational_sem_lev_goal.
 
